@prefix rdf:                <http://www.w3.org/1999/02/22-rdf-syntax-ns#> .
@prefix skos:               <http://www.w3.org/2004/02/skos/core#> .

# --- Own namespaces ------------------------

@prefix code:               <http://stats.govdata.ie/codelist/> .
@prefix code-residence:     <http://stats.govdata.ie/codelist/usual-residence/> .

#Â --- Code list -----------------------------

code:usual-residence a skos:ConceptScheme;
    skos:prefLabel "Code list for usual residences"@en;
    skos:hasTopConcept code-residence:same-address,
      code-residence:elsewhere-in-county,
      code-residence:elsewhere-in-ireland,
      code-residence:outside-ireland,
      code-residence:total
    .

code-residence:same-address a skos:Concept;
    skos:inScheme code:usual-residence;
    skos:topConceptOf code:usual-residence;
    skos:prefLabel "Same address"@en;
    skos:definition "The person is usually resident in the same geographic area where the statistical data was collected."@en;
    skos:broader code-residence:total
    .

code-residence:elsewhere-in-county a skos:Concept;
    skos:inScheme code:usual-residence;
    skos:topConceptOf code:usual-residence;
    skos:prefLabel "Elsewhere in County"@en;
    skos:definition "The person has usual residence in other part of the county than the part for which the statistical data was collected."@en;
    skos:broader code-residence:total
    .

code-residence:elsewhere-in-ireland a skos:Concept;
    skos:inScheme code:usual-residence;
    skos:topConceptOf code:usual-residence;
    skos:prefLabel "Elsewhere in Ireland"@en;
    skos:definition "The person has usual residence in other part of Ireland than the part for which the statistical data was collected."@en;
    skos:broader code-residence:total
    .

code-residence:outside-ireland a skos:Concept;
    skos:inScheme code:usual-residence;
    skos:topConceptOf code:usual-residence;
    skos:prefLabel "Outside Ireland"@en;
    skos:definition "The person's usual residence is outside of Ireland."@en;
    skos:broader code-residence:total
    .

code-residence:total a skos:Concept;
    skos:inScheme code:usual-residence;
    skos:topConceptOf code:usual-residence;
    skos:prefLabel "Total"@en;
    skos:narrower code-residence:same-address,
      code-residence:elsewhere-in-county,
      code-residence:elsewhere-in-ireland,
      code-residence:outside-ireland
    .
